coq: STLC

coq/Logic/STLC/Example.v
@@ -1,3 +1,5 @@
+Require Import List.
+
 Require Import Logic.Class.Eq.
 
 Require Import Logic.STLC.Eval.
@@ -6,26 +8,60 @@ Require Import Logic.STLC.Subst.
 Require Import Logic.STLC.Syntax.
 Require Import Logic.STLC.Replace.
 
-Definition id (b v:Type)(x:v) : Exp b v := 
-    Lam x (Var x). 
+Definition id (b v:Type)(x:v) : Exp b v := \x ~> `x.
 
 Arguments id {b} {v}.
 
-Definition const (b v:Type) (x y:v) : Exp b v :=
-    Lam x (Lam y (Var x)).
+(* This will not have the right semantics unless x and y are distinct           *)
+Definition const (b v:Type) (x y:v) : Exp b v := \x ~> \y ~> `x.
 
 Arguments const {b} {v}.
 
+(* Annotated identity applied to variable y reduces to variable y               *)
 Lemma idAnn : forall (b v:Type) (e:Eq v) (x y:v) (a:T b),
-    Eval (App (Ann (id x) (Fun a a)) (Var y)) (Var y).
+    (id x :: a :-> a) $ `y >> `y.
 Proof.
-    intros b v e x y a. apply (EAppL (Ann (id x) (Fun a a)) (Var x) _ _ x).
+    intros b v e x y a. apply (EAppL (id x :: a :-> a) `x _ _ x).
     - apply VVar.
     - apply VVar.
     - constructor. apply VLam, VVar. apply ELam.
         + apply VVar.
         + constructor.
     - rewrite substVar. rewrite replace_x. constructor.
+Qed.
+
+(* Annotated const applied to identity and variable u reduces to identity       *)
+(* Note that we need the variables x and y to be distinct for this to hold      *)
+Lemma constAnn : forall (base v:Type) (e:Eq v) (x y z u:v) (a b : T base),
+    x <> y -> (const x y :: (b :-> b) :-> a :-> b :-> b) $ (id z) $ `u >> id z. 
+Proof.
+    intros base v e x y z u a b H1. apply (EAppL _ (id z) _ _ y).
+    - apply VLam, VVar.
+    - apply VLam, VVar.
+    - apply (EAppL _ (\y ~> `x) _ _ x). 
+        + apply VLam, VVar.
+        + apply VLam, VLam, VVar.
+        + constructor.
+            { apply VLam, VLam, VVar. }
+            { constructor.
+                { apply VLam, VVar. }
+                { constructor.
+                    { apply VVar. }
+                    { constructor. }}}
+        + constructor. 
+            { apply VLam, VVar. }
+            { destruct (in_dec eqDec x (y :: nil)) as [H2|H2].
+                { exfalso. destruct H2 as [H2|H2].
+                    { auto. }
+                    { inversion H2. }}
+                { rewrite replace_x. apply ELam.
+                    { apply VVar. }
+                    { apply EVar. }}}
+    - apply ELam.
+        + apply VVar.
+        + destruct (in_dec eqDec z (z :: nil)) as [H2|H2].
+            { apply EVar. }
+            { exfalso. apply H2. left. reflexivity. }
 Qed.
 
 
