coq/Logic/STLC/Context.v
@@ -1,0 +1,148 @@
+Require Import Logic.Class.Eq.
+
+Require Import Logic.STLC.Syntax.
+
+Inductive Binding (b v:Type) : Type :=
+| BType : b -> Binding b v          (* Adding base type to context              *)
+| BVar  : v -> T b -> Binding b v   (* Adding variable to context               *)
+.
+
+Arguments Binding {b} {v}.
+Arguments BType   {b} {v}.
+Arguments BVar    {b} {v}.
+
+Notation "Ty ::: *" := (BType Ty)
+    (at level 1, no associativity)      : STLC_Context_scope.
+
+Notation "x ::: Ty" :=(BVar x Ty)
+    (at level 1, no associativity)      : STLC_Context_scope.
+
+
+Inductive Context (b v:Type) : Type :=
+| O         : Context b v
+| CtxSnoc   : Context b v -> @Binding b v -> Context b v
+.
+
+Arguments Context {b} {v}.
+Arguments O       {b} {v}.
+Arguments CtxSnoc {b} {v}.
+
+Notation "G ; x" := (CtxSnoc G x)
+    (at level 50, left associativity) : STLC_Context_scope.
+
+Open Scope STLC_Context_scope.
+
+Inductive FindTy (b v:Type) : @Context b v -> b -> Prop :=
+| FindTyZ : forall (G:Context) (Ty:b), FindTy b v (G ; Ty ::: *) Ty
+| FindTyS : forall (G:Context) (Ty:b) (k:Binding),
+    FindTy b v G Ty -> FindTy b v (G ; k) Ty
+.
+
+Arguments FindTy  {b} {v}.
+Arguments FindTyZ {b} {v}.
+Arguments FindTyS {b} {v}.
+
+
+
+Notation "G :> Ty" := (FindTy G Ty)
+    (at level 60, no associativity) : STLC_Context_scope.
+
+Lemma findTyRev : forall (b v:Type) (G:Context) (x:v) (Sy:T b) (Ty : b),
+    G ; x ::: Sy :> Ty -> G :> Ty.
+Proof.
+    intros b v G x Sy Ty H1. remember (G ; x ::: Sy) as G' eqn:E.
+    revert G x Sy E. destruct H1 as [G Ty|G Ty k H1]; intros G' x Sy H2.
+    - inversion H2. 
+    - inversion H2. subst. assumption.
+Qed.
+
+
+Inductive FindVar (b v:Type) (e:Eq v) : @Context b v -> @Binding b v -> Prop :=
+| FindVarZ : forall (G:Context) (x:v) (Ty:T b), 
+    FindVar b v e (G ; x ::: Ty) (x ::: Ty)
+| FindVarSkip : forall (G:Context) (k:Binding) (Ty:b),
+    FindVar b v e G k -> FindVar b v e (G ; Ty ::: * ) k
+| FindVarS : forall (G:Context) (x y:v) (Ty Sy:T b),
+    x <> y                                  ->
+    FindVar b v e G (x ::: Ty)              ->
+    FindVar b v e (G ; y ::: Sy) (x ::: Ty)
+.
+
+Arguments FindVar     {b} {v} {e}.
+Arguments FindVarZ    {b} {v} {e}.
+Arguments FindVarSkip {b} {v} {e}.
+Arguments FindVarS    {b} {v} {e}.
+
+Notation "G :>> k" := (FindVar G k)
+    (at level 60, no associativity) : STLC_Context_scope.
+
+Lemma findVarRev : forall (b v:Type) (e:Eq v) (G:Context) (Sy:b) (x:v) (Ty:T b),
+    G ; Sy ::: * :>> x ::: Ty -> G :>> x ::: Ty.
+Proof.
+    intros b v e G Sy x Ty H1.
+    remember (G ; Sy ::: *) as G' eqn:E. remember (x ::: Ty) as k eqn:F.
+    revert G Sy x Ty E F. destruct H1 as [G x Ty|G k Ty H1|G x y Ty Uy H1 H2];
+    intros G' Sy x' Ty' H3 H4. 
+    - inversion H3.
+    - inversion H3. subst. assumption.
+    - inversion H3.
+Qed.
+
+Definition ctxIncl (b v:Type)(e:Eq v)(G H:@Context b v) : Prop :=
+    (forall (Ty:b), G :> Ty -> H :> Ty) /\
+    (forall (x:v) (Ty:T b), G :>> x ::: Ty -> H :>> x ::: Ty).
+
+Arguments ctxIncl {b} {v} {e}.
+
+Notation "G <= H"  := (ctxIncl G H)
+    (at level 70, no associativity) : STLC_Context_scope.
+
+Open Scope STLC_Context_scope.
+
+Lemma ctxInclO : forall (b v:Type) (e:Eq v) (G:@Context b v), 
+    O <= G.
+Proof.
+    intros b v e G. split.
+    - intros Ty H1. remember O as H eqn:E. revert G E.
+      induction H1 as [G Ty|G Ty k H1 IH]; intros G' H2; inversion H2.
+    - intros x Ty H1. remember (x ::: Ty) as k eqn:E. 
+      remember O as H eqn:F. revert G x Ty E F.
+      induction H1 as [G x Ty|G k Ty H1 IH|G x y Ty Sy H1 H2 IH];
+      intros G' x' Ty' H3 H4; inversion H4.
+Qed.
+
+Lemma ctxInclRefl : forall (b v:Type) (e:Eq v) (G:@Context b v), 
+    G <= G.
+Proof. intros b v e G. split; auto. Qed.
+
+Lemma ctxInclTrans : forall (b v:Type) (e:Eq v) (G H K:@Context b v),
+    G <= H -> H <= K -> G <= K.
+Proof. intros b v e G H K [H1 H2] [H3 H4]. split; auto. Qed.
+
+Lemma ctxInclExtendTy : forall (b v:Type) (e:Eq v) (G H:@Context b v) (Ty:b),
+    G <= H -> G ; Ty ::: * <= H ; Ty ::: *.
+Proof.
+    intros b v e G H Ty [H1 H2]. split.
+    - intros Ty' H3.  remember (G ; Ty ::: * ) as G' eqn:E.
+      revert G H H1 H2 Ty E. destruct H3 as [G Ty|G Ty k H1].
+        + intros G' H H2 H3 Ty' H4. inversion H4. apply FindTyZ.
+        + intros G' H H2 H3 Ty' H4. inversion H4. subst.
+          apply FindTyS, H2. assumption.
+    - intros x Ty' H3. constructor. apply H2. apply findVarRev in H3. assumption.
+Qed.
+
+Lemma ctxInclExtendVar : forall (b v:Type)(e:Eq v)(G H:@Context b v)(x:v)(Ty:T b),
+    G <= H -> G ; x ::: Ty <= H ; x ::: Ty.
+Proof.
+    intros b v e G H x Ty [H1 H2]. split.
+    - intros Sy H3. apply FindTyS, H1. apply findTyRev in H3. assumption.
+    - intros x' Ty' H3.
+      remember (G ; x ::: Ty) as G' eqn:E. remember (x' ::: Ty') as k eqn:F.
+      revert G H x Ty H1 H2 x' Ty' E F.
+      destruct H3 as [G x Ty|G k Ty H1|G x y Ty Sy H1 H2];
+      intros G' H x' Ty' H3 H4 y' Sy' H5 H6. 
+        + inversion H5. apply FindVarZ.
+        + inversion H5.
+        + inversion H5. subst. apply FindVarS; try assumption. 
+          apply H4. assumption.
+Qed.
