coq/Logic/STLC/IsType.v
@@ -1,0 +1,21 @@
+Require Import Logic.STLC.Syntax.
+Require Import Logic.STLC.Context.
+
+Inductive IsType (b v:Type) : @Context b v -> T b -> Prop :=
+| TVar : forall (G:Context) (Ty:b), 
+    G :> Ty -> 
+    IsType b v G (Base Ty)  
+| TFun : forall (G:Context) (Ty Ty':T b),
+    IsType b v G Ty     -> 
+    IsType b v G Ty'    -> 
+    IsType b v G (Ty :-> Ty') 
+.
+
+Arguments IsType {b} {v}.
+Arguments TVar   {b} {v}.
+Arguments TFun   {b} {v}.
+
+Notation "G :- Ty" := (IsType G Ty)
+    (at level 1, no associativity) : STLC_IsType_scope.
+
+Open Scope STLC_IsType_scope.
