coq/Logic/STLC/Valid.v
@@ -1,0 +1,38 @@
+Require Import Logic.STLC.Syntax.
+Require Import Logic.STLC.IsType.
+Require Import Logic.STLC.Context.
+
+Inductive Valid (b v:Type) : @Context b v -> Prop :=
+| ValidO   : Valid b v O
+| ValidTy  : forall (G:Context) (Ty:b),
+    Valid b v G -> Valid b v (G ; Ty ::: *)
+| ValidVar : forall (G:Context) (x:v) (Ty:T b),
+    Valid b v G -> G :- Ty -> Valid b v (G ; x ::: Ty) 
+.
+
+Arguments Valid    {b} {v}.
+Arguments ValidO   {b} {v}.
+Arguments ValidTy  {b} {v}.
+Arguments ValidVar {b} {v}.
+
+(* An example of valid context                                                  *)
+Definition G1 (base v:Type) (a b:base) (const:v) : @Context base v 
+    := O
+    ; a ::: *
+    ; b ::: *
+    ; const ::: ((Base b :-> Base b) :-> Base a :-> Base b :-> Base b)
+    .
+Arguments G1 {base} {v}.
+
+Lemma ValidG1 : forall (base v:Type) (a b:base) (const:v),
+    Valid (G1 a b const).
+Proof.
+    intros base v a b const. constructor.
+    - constructor. constructor. constructor.
+    - constructor.
+        + constructor; constructor; apply FindTyZ.
+        + constructor.
+            { constructor. apply FindTyS, FindTyZ. }
+            { constructor; constructor; apply FindTyZ. }
+Qed.
+
